code/ecdsap256/Hacl.Impl.ScalarMultiplication.Ladder.fst
@@ -1,0 +1,291 @@
+module Hacl.Impl.ScalarMultiplication.Ladder
+
+open FStar.HyperStack.All
+open FStar.HyperStack
+module ST = FStar.HyperStack.ST
+
+open Lib.IntTypes
+open Lib.Buffer
+open Lib.Loops
+
+open Spec.P256
+open Spec.P256.Lemmas
+open Spec.P256.Definitions
+
+open Spec.P256.MontgomeryMultiplication
+open Hacl.Impl.P256.MontgomeryMultiplication
+
+open Hacl.Impl.P256.PointAdd
+open Hacl.Impl.P256.PointDouble
+
+open FStar.Mul
+
+
+val swap: p: point_prime -> q: point_prime -> 
+  Tot (r: tuple2 point_prime point_prime {let pNew, qNew = r in pNew == q /\ qNew == p})
+
+let swap p q = (q, p)
+
+
+val conditional_swap: i: uint64 -> p: point_prime -> q: point_prime -> 
+  Tot (r: tuple2 point_prime point_prime {
+    let pNew, qNew = r in 
+    if uint_v i = 0 then pNew == p /\ qNew == q
+    else
+      let p1, q1 = swap p q in 
+      p1 == pNew /\ q1 == qNew}
+  )
+
+let conditional_swap i p q = 
+  if uint_v i = 0 then 
+    (p, q)
+  else
+    (q, p)
+
+
+[@ CInline]
+val cswap: bit:uint64{v bit <= 1} -> p:point -> q:point -> 
+  Stack unit
+  (requires fun h ->
+    live h p /\ live h q /\ (disjoint p q \/ p == q) /\
+           
+    as_nat h (gsub p (size 0) (size 4)) < prime /\ 
+    as_nat h (gsub p (size 4) (size 4)) < prime /\
+    as_nat h (gsub p (size 8) (size 4)) < prime /\
+       
+    as_nat h (gsub q (size 0) (size 4)) < prime /\  
+    as_nat h (gsub q (size 4) (size 4)) < prime /\
+    as_nat h (gsub q (size 8) (size 4)) < prime
+  )
+  (ensures  fun h0 _ h1 ->
+    modifies (loc p |+| loc q) h0 h1 /\ (
+    let pBefore = as_seq h0 p in let qBefore = as_seq h0 q in 
+    let pAfter = as_seq h1 p in let qAfter = as_seq h1 q in 
+    let condP0, condP1 = conditional_swap bit pBefore qBefore  in 
+    condP0 == pAfter /\ condP1 == qAfter) /\ (
+    v bit == 1 ==> as_seq h1 p == as_seq h0 q /\ as_seq h1 q == as_seq h0 p) /\ (
+    v bit == 0 ==> as_seq h1 p == as_seq h0 p /\ as_seq h1 q == as_seq h0 q)
+  )
+
+
+let cswap bit p1 p2 =
+  let open Lib.Sequence in 
+  let h0 = ST.get () in
+  let mask = u64 0 -. bit in
+
+  [@ inline_let]
+  let inv h1 (i:nat{i <= 12}) =
+    (forall (k:nat{k < i}).
+      if v bit = 1
+      then (as_seq h1 p1).[k] == (as_seq h0 p2).[k] /\ (as_seq h1 p2).[k] == (as_seq h0 p1).[k]
+      else (as_seq h1 p1).[k] == (as_seq h0 p1).[k] /\ (as_seq h1 p2).[k] == (as_seq h0 p2).[k]) /\
+    (forall (k:nat{i <= k /\ k < 12}).
+      (as_seq h1 p1).[k] == (as_seq h0 p1).[k] /\ (as_seq h1 p2).[k] == (as_seq h0 p2).[k]) /\
+    modifies (loc p1 |+| loc p2) h0 h1 in
+ 
+  Lib.Loops.for 0ul 12ul inv
+    (fun i ->
+      let dummy = mask &. (p1.(i) ^. p2.(i)) in
+      p1.(i) <- p1.(i) ^. dummy;
+      p2.(i) <- p2.(i) ^. dummy;
+      lemma_cswap2_step bit ((as_seq h0 p1).[v i]) ((as_seq h0 p2).[v i])
+    );
+  let h1 = ST.get () in
+  Lib.Sequence.eq_intro (as_seq h1 p1) (if v bit = 1 then as_seq h0 p2 else as_seq h0 p1);
+  Lib.Sequence.eq_intro (as_seq h1 p2) (if v bit = 1 then as_seq h0 p1 else as_seq h0 p2)
+
+
+(* this piece of code is taken from Hacl.Curve25519 *)
+(* changed Endian for Scalar Bit access *)
+inline_for_extraction noextract
+val scalar_bit:
+    #buf_type: buftype -> 
+    s:lbuffer_t buf_type uint8 (size 32)
+  -> n:size_t{v n < 256}
+  -> Stack uint64
+    (requires fun h0 -> live h0 s)
+    (ensures  fun h0 r h1 -> h0 == h1 /\ r == ith_bit (as_seq h0 s) (v n) /\ v r <= 1)
+
+let scalar_bit #buf_type s n =
+  let h0 = ST.get () in
+  mod_mask_lemma ((Lib.Sequence.index (as_seq h0 s) (31 - v n / 8)) >>. (n %. 8ul)) 1ul;
+  assert_norm (1 = pow2 1 - 1);
+  assert (v (mod_mask #U8 #SEC 1ul) == v (u8 1)); 
+  to_u64 ((s.(31ul -. n /. 8ul) >>. (n %. 8ul)) &. u8 1)
+
+
+inline_for_extraction noextract  
+val montgomery_ladder_step1: p: point -> q: point ->tempBuffer: lbuffer uint64 (size 88) -> 
+  Stack unit
+  (requires fun h -> live h p /\ live h q /\ live h tempBuffer /\ 
+    LowStar.Monotonic.Buffer.all_disjoint [loc p; loc q; loc tempBuffer] /\
+
+    as_nat h (gsub p (size 0) (size 4)) < prime /\ 
+    as_nat h (gsub p (size 4) (size 4)) < prime /\
+    as_nat h (gsub p (size 8) (size 4)) < prime /\
+  
+    as_nat h (gsub q (size 0) (size 4)) < prime /\  
+    as_nat h (gsub q (size 4) (size 4)) < prime /\
+    as_nat h (gsub q (size 8) (size 4)) < prime
+  )
+  (ensures fun h0 _ h1 -> modifies (loc p |+| loc q |+|  loc tempBuffer) h0 h1 /\ (
+    let pX = as_nat h0 (gsub p (size 0) (size 4)) in
+    let pY = as_nat h0 (gsub p (size 4) (size 4)) in
+    let pZ = as_nat h0 (gsub p (size 8) (size 4)) in
+
+    let qX = as_nat h0 (gsub q (size 0) (size 4)) in
+    let qY = as_nat h0 (gsub q (size 4) (size 4)) in
+    let qZ = as_nat h0 (gsub q (size 8) (size 4)) in
+
+    let r0X = as_nat h1 (gsub p (size 0) (size 4)) in
+    let r0Y = as_nat h1 (gsub p (size 4) (size 4)) in
+    let r0Z = as_nat h1 (gsub p (size 8) (size 4)) in
+
+    let r1X = as_nat h1 (gsub q (size 0) (size 4)) in
+    let r1Y = as_nat h1 (gsub q (size 4) (size 4)) in
+    let r1Z = as_nat h1 (gsub q (size 8) (size 4)) in
+
+    let (rN0X, rN0Y, rN0Z), (rN1X, rN1Y, rN1Z) = _ml_step1 (fromDomain_ pX, fromDomain_ pY, fromDomain_ pZ) (fromDomain_ qX, fromDomain_ qY, fromDomain_ qZ) in     
+    fromDomain_ r0X == rN0X /\ fromDomain_ r0Y == rN0Y /\ fromDomain_ r0Z == rN0Z /\
+    fromDomain_ r1X == rN1X /\ fromDomain_ r1Y == rN1Y /\ fromDomain_ r1Z == rN1Z /\ 
+
+    r0X < prime /\ r0Y < prime /\ r0Z < prime /\
+    r1X < prime /\ r1Y < prime /\ r1Z < prime) 
+  )
+
+
+let montgomery_ladder_step1 r0 r1 tempBuffer = 
+  point_add r0 r1 r1 tempBuffer;
+  point_double r0 r0 tempBuffer
+      
+
+val lemma_step: i: size_t {uint_v i < 256} -> Lemma  (uint_v ((size 255) -. i) == 255 - (uint_v i))
+let lemma_step i = ()
+
+
+inline_for_extraction noextract 
+val montgomery_ladder_step: #buf_type: buftype-> 
+  p: point -> q: point ->tempBuffer: lbuffer uint64 (size 88) -> 
+  scalar: lbuffer_t buf_type uint8 (size 32) -> 
+  i:size_t{v i < 256} -> 
+  Stack unit
+  (requires fun h -> live h p /\ live h q /\ live h tempBuffer /\ live h scalar /\
+    LowStar.Monotonic.Buffer.all_disjoint [loc p; loc q; loc tempBuffer; loc scalar] /\
+     
+    as_nat h (gsub p (size 0) (size 4)) < prime /\ 
+    as_nat h (gsub p (size 4) (size 4)) < prime /\
+    as_nat h (gsub p (size 8) (size 4)) < prime /\
+  
+    as_nat h (gsub q (size 0) (size 4)) < prime /\  
+    as_nat h (gsub q (size 4) (size 4)) < prime /\
+    as_nat h (gsub q (size 8) (size 4)) < prime
+  )
+  (ensures fun h0 _ h1 -> modifies (loc p |+| loc q |+| loc tempBuffer) h0 h1 /\ (
+      
+      let pX = as_nat h0 (gsub p (size 0) (size 4)) in
+      let pY = as_nat h0 (gsub p (size 4) (size 4)) in
+      let pZ = as_nat h0 (gsub p (size 8) (size 4)) in
+
+      let qX = as_nat h0 (gsub q (size 0) (size 4)) in
+      let qY = as_nat h0 (gsub q (size 4) (size 4)) in
+      let qZ = as_nat h0 (gsub q (size 8) (size 4)) in
+
+      let r0X = as_nat h1 (gsub p (size 0) (size 4)) in
+      let r0Y = as_nat h1 (gsub p (size 4) (size 4)) in
+      let r0Z = as_nat h1 (gsub p (size 8) (size 4)) in
+
+      let r1X = as_nat h1 (gsub q (size 0) (size 4)) in
+      let r1Y = as_nat h1 (gsub q (size 4) (size 4)) in
+      let r1Z = as_nat h1 (gsub q (size 8) (size 4)) in
+
+      let (rN0X, rN0Y, rN0Z), (rN1X, rN1Y, rN1Z) = _ml_step (as_seq h0 scalar) (uint_v i) ((fromDomain_ pX, fromDomain_ pY, fromDomain_ pZ), (fromDomain_ qX, fromDomain_ qY, fromDomain_ qZ)) in 
+      
+      fromDomain_ r0X == rN0X /\ fromDomain_ r0Y == rN0Y /\ fromDomain_ r0Z == rN0Z /\
+      fromDomain_ r1X == rN1X /\ fromDomain_ r1Y == rN1Y /\ fromDomain_ r1Z == rN1Z /\ 
+
+      r0X < prime /\ r0Y < prime /\ r0Z < prime /\
+      r1X < prime /\ r1Y < prime /\ r1Z < prime
+    ) 
+  )
+
+
+let montgomery_ladder_step #buf_type r0 r1 tempBuffer scalar i = 
+  let bit0 = (size 255) -. i in 
+  let bit = scalar_bit scalar bit0 in 
+  cswap bit r0 r1; 
+  montgomery_ladder_step1 r0 r1 tempBuffer; 
+  cswap bit r0 r1; 
+    lemma_step i
+
+
+
+
+inline_for_extraction noextract
+val montgomery_ladder: #buf_type: buftype->  p: point -> q: point ->
+  scalar: lbuffer_t buf_type uint8 (size 32) -> 
+  tempBuffer:  lbuffer uint64 (size 88)  -> 
+  Stack unit
+  (requires fun h -> live h p /\ live h q /\ live h scalar /\  live h tempBuffer /\
+    LowStar.Monotonic.Buffer.all_disjoint [loc p; loc q; loc tempBuffer; loc scalar] /\
+    as_nat h (gsub p (size 0) (size 4)) < prime /\ 
+    as_nat h (gsub p (size 4) (size 4)) < prime /\
+    as_nat h (gsub p (size 8) (size 4)) < prime /\
+  
+    as_nat h (gsub q (size 0) (size 4)) < prime /\  
+    as_nat h (gsub q (size 4) (size 4)) < prime /\
+    as_nat h (gsub q (size 8) (size 4)) < prime )
+  (ensures fun h0 _ h1 -> modifies (loc p |+| loc q |+| loc tempBuffer) h0 h1 /\
+    (
+      as_nat h1 (gsub p (size 0) (size 4)) < prime /\ 
+      as_nat h1 (gsub p (size 4) (size 4)) < prime /\
+      as_nat h1 (gsub p (size 8) (size 4)) < prime /\
+  
+      as_nat h1 (gsub q (size 0) (size 4)) < prime /\  
+      as_nat h1 (gsub q (size 4) (size 4)) < prime /\
+      as_nat h1 (gsub q (size 8) (size 4)) < prime /\
+
+
+      (
+  let p1 = fromDomainPoint(point_prime_to_coordinates (as_seq h1 p)) in 
+  let q1 = fromDomainPoint(point_prime_to_coordinates (as_seq h1 q)) in 
+  let rN, qN = montgomery_ladder_spec (as_seq h0 scalar) 
+    (
+      fromDomainPoint(point_prime_to_coordinates (as_seq h0 p)),  
+      fromDomainPoint(point_prime_to_coordinates (as_seq h0 q))
+    ) in 
+  rN == p1 /\ qN == q1
+      )
+   )
+ )
+
+let montgomery_ladder #a p q scalar tempBuffer =  
+  let h0 = ST.get() in 
+
+
+  [@inline_let]
+  let spec_ml h0 = _ml_step (as_seq h0 scalar) in 
+
+  [@inline_let] 
+  let acc (h:mem) : GTot (tuple2 point_nat_prime point_nat_prime) = 
+  (fromDomainPoint(point_prime_to_coordinates (as_seq h p)), fromDomainPoint(point_prime_to_coordinates (as_seq h q)))  in 
+  
+  Lib.LoopCombinators.eq_repeati0 256 (spec_ml h0) (acc h0);
+  [@inline_let]
+  let inv h (i: nat {i <= 256}) = 
+    as_nat h (gsub p (size 0) (size 4)) < prime /\ 
+    as_nat h (gsub p (size 4) (size 4)) < prime /\
+    as_nat h (gsub p (size 8) (size 4)) < prime /\
+  
+    as_nat h (gsub q (size 0) (size 4)) < prime /\  
+    as_nat h (gsub q (size 4) (size 4)) < prime /\
+    as_nat h (gsub q (size 8) (size 4)) < prime /\
+    modifies3 p q tempBuffer h0 h   /\
+    acc h == Lib.LoopCombinators.repeati i (spec_ml h0) (acc h0)
+
+    in 
+
+  for 0ul 256ul inv 
+    (fun i -> let h2 = ST.get() in
+      montgomery_ladder_step p q tempBuffer scalar i; 
+      Lib.LoopCombinators.unfold_repeati 256 (spec_ml h0) (acc h0) (uint_v i)
+    )
