code/ecdsap256/Hacl.Impl.ScalarMultiplication.Radix4.fst
@@ -1,0 +1,384 @@
+module Hacl.Impl.ScalarMultiplication.Radix4
+
+open FStar.HyperStack.All
+open FStar.HyperStack
+module ST = FStar.HyperStack.ST
+
+open Lib.IntTypes
+open Lib.Buffer
+open Lib.Loops
+
+open Spec.P256
+open Spec.P256.Lemmas
+open Spec.P256.Definitions
+
+open Spec.P256.MontgomeryMultiplication
+open Hacl.Impl.P256.MontgomeryMultiplication
+
+open Hacl.Impl.P256.LowLevel
+open Hacl.Impl.P256.PointAdd
+open Hacl.Impl.P256.PointDouble
+
+open FStar.Mul
+
+open Hacl.Impl.P256.Q.PrimitivesMasking
+
+
+
+(* prime = 2**256 - 2**224 + 2**192 + 2**96 -1
+
+def norm(p):    
+    x, y, z = p
+    z2i = power_mod(z * z, -1, prime)
+    z3i = power_mod(z * z * z, -1, prime)
+    return ((x * z2i) % prime, (y * z3i) % prime, 1)
+
+def toD(x):
+    return x * power_mod (2 ** 256, 1, prime) % prime
+
+def fromD(x):
+    return x * power_mod (2 ** 256, prime - 2, prime) % prime
+
+def toFakeAffine(p):
+    x, y = p 
+    multiplier = power_mod (2 ** 256, prime - 2, prime) 
+    x = x * multiplier * multiplier % prime
+    y = y * multiplier * multiplier * multiplier % prime
+    return (x, y)
+
+p256 = 0xFFFFFFFF00000001000000000000000000000000FFFFFFFFFFFFFFFFFFFFFFFF
+a256 = p256 - 3
+b256 = 0x5AC635D8AA3A93E7B3EBBD55769886BC651D06B0CC53B0F63BCE3C3E27D2604B
+gx = 0x6B17D1F2E12C4247F8BCE6E563A440F277037D812DEB33A0F4A13945D898C296
+gy = 0x4FE342E2FE1A7F9B8EE7EB4A7C0F9E162BCE33576B315ECECBB6406837BF51F5
+qq = 0xFFFFFFFF00000000FFFFFFFFFFFFFFFFBCE6FAADA7179E84F3B9CAC2FC632551
+FF = GF(p256)
+
+EC = EllipticCurve([FF(a256), FF(b256)])
+
+EC.set_order(qq)
+
+G = EC(FF(gx), FF(gy))
+
+def printf(p):
+    x, y = p 
+    for i in range(4):
+        print("u64 " + str(hex((Integer(x) >> (i * 64)) % 2 ** 64)) + "; ")
+    for i in range(4):
+        print("u64 " + str (hex((Integer(y) >> (i * 64)) % 2 ** 64)) + "; ")
+    
+
+for i in range(16):
+    pxD = i * G.xy()[0]
+    pyD = i * G.xy()[1]
+    printf (toFakeAffine((to D (pxD), toD (pyD))))
+
+ *)
+
+inline_for_extraction noextract
+let points_radix_16_list : x:list uint64{List.Tot.length x == 128} =
+  let open FStar.Mul in 
+  [@inline_let]
+  let x = [ 
+    u64 0x0; u64 0x0; u64 0x0; u64 0x0; 
+    u64 0x0; u64 0x0; u64 0x0; u64 0x0; 
+
+    u64 0x1fb38ab1388ad777; u64 0x1dfee06615fa309d; u64 0xfcac986c3afea4a7; u64 0xdf65c2da29fb821a; 
+    u64 0xeff44e23f63f8f6d; u64 0xaa02cd3ed4b681a4; u64 0xdd5fda3363818af8; u64 0xfc53bc2629fbf0b3; 
+
+    u64 0x12631d721b91beea; u64 0x5f73f2d3a11a09f8; u64 0xac41f54484d5fcd8; u64 0x86578e5c56025df4; 
+    u64 0x577c956b15ed6b5a; u64 0xb59c5f77982d848; u64 0xb7c5e2c190fcdcc2; u64 0x7d64d13ef1c91ffd; 
+
+    u64 0xd40c2d6273f9d9f1; u64 0x4dc6f628063ef17c; u64 0x498e81df7ab17aa5; u64 0xabb2a5026f17173c; 
+    u64 0x4a3d7527f6739ef3; u64 0xd941003268184c91; u64 0xd2d458b8d401508b; u64 0xb7437ab810ac5451; 
+
+    u64 0x5256d9bdab491252; u64 0x972d326eb1084c12; u64 0xc3e96455e2ec3bfa; u64 0xb75c723b549a10ff; 
+    u64 0x9d9185f9f8a18961; u64 0x2200a07b8589ba82; u64 0x637b9d96fd4e9f5e; u64 0xce75bfb2575e6cfa; 
+
+    u64 0x7dd4477db8b77c7d; u64 0x80818a776e5503b0; u64 0x6fc7d58fb59581d; u64 0xd899fb87efe43022; 
+    u64 0x23b9912111694135; u64 0x7e5de7bac33fa1c8; u64 0xb3b83722a70e7d43; u64 0xf06cfecbfb9bb38f; 
+
+    u64 0xaa39277dfa93656; u64 0x3dabb6cce67c5201; u64 0x473ffb8bf1f94677; u64 0xb9f0b93637453e56; 
+    u64 0x8fce12ec20958fb2; u64 0xcc16d74ff7786061; u64 0x3678438a8235d096; u64 0xe39ea044f06b43f6; 
+
+    u64 0xbb40bdb5775c9950; u64 0xd244a74cdc703cdd; u64 0x83dc1b8a6105dd53; u64 0x38d9d50d49ef0437; 
+    u64 0x58be44eba6096472; u64 0x960afaec386fa5c5; u64 0x1440032e000134b9; u64 0x601e721454d6ba96; 
+
+    u64 0x79ec42228671b9b6; u64 0xfdc00dc48df9e25c; u64 0x44500833d71d2e77; u64 0x2bda4c3c0bc103d5; 
+    u64 0x51528408aa925d53; u64 0xefcb55b9c2f3a37d; u64 0x9f28f6bb9846c915; u64 0xe1547ce1d8340e55; 
+
+    u64 0x97e310c1995b3ed2; u64 0xed861937196256e6; u64 0x1c6762abff2c65f2; u64 0x268345e0978fcedd; 
+    u64 0x35ca2e572b784881; u64 0x28ac888da0acd1b7; u64 0x305640dc06a41baf; u64 0x997c6fd2cb671bfb; 
+
+    u64 0xf40d9eaf4a31e15a; u64 0x8991dd7d54cfe03a; u64 0x4889a3463a8deb0c; u64 0x4cbf48092cd0a1fa; 
+    u64 0xc6965c4fbe18fb8c; u64 0x1d499d0cb216fa84; u64 0x8d5fe52c705dd3eb; u64 0x812b268f84313b34; 
+
+    u64 0x313b58808261591a; u64 0xc2c322508f53d933; u64 0xa49ef3f95094ed1b; u64 0x13e326786e98c63; 
+    u64 0x34be8167cd460429; u64 0x698a328099a6b31; u64 0xb9be3ba51b0c922d; u64 0xe59cca03f7674ed; 
+    
+    u64 0x4fbf7e505d3aca7c; u64 0x2f4f8ba62020715; u64 0x840502262ac1ec42; u64 0xb8e0532775197de7; 
+    u64 0x9142a358cf4e9b4b; u64 0xc86a3c567e5d8626; u64 0xd4051282b4a7992a; u64 0xe7573c5999e3974e;
+    
+    u64 0xd814a606da7bd76b; u64 0x15604730f38cb788; u64 0xbd195f868fbdd6c4; u64 0xdb96f5b00a51d3f7; 
+    u64 0xe1385c8a9b507fea; u64 0x878e27813ee7310; u64 0x6d7d8b12aea7e096; u64 0x54978ad11e2f5cca; 
+    
+    u64 0x49fffd6c3c4d07d4; u64 0x703638f71fab7a5d; u64 0xbed6e367fcc73960; u64 0x215e161835a61d75; 
+    u64 0xe52288a5e87a660b; u64 0xf1d127ee3c802cb5; u64 0xccde3c6aafc46044; u64 0xdc11c08ef14cff32; 
+
+    u64 0x29216f9ceca46668; u64 0x22e584a3b2891c5e; u64 0xe6deecd7810f6d87; u64 0x6aff4b94a55659a3; 
+   u64 0x12b59bb6d2e9f876; u64 0x27ed01943aa02eab; u64 0x8d6d420841f57075; u64 0xe7b47285ef60a461;  
+  ] in x
+
+
+
+
+inline_for_extraction
+let points_radix_16 : x: glbuffer uint64 128ul {witnessed #uint64 #(size 128) x (Lib.Sequence.of_list points_radix_16_list) /\ recallable x} =
+    createL_global points_radix_16_list
+
+
+
+[@ CInline]
+inline_for_extraction noextract  
+val getScalar: #buf_type: buftype -> scalar: lbuffer_t buf_type uint8 (size 32) -> i: size_t {v i < 64} -> 
+  Stack uint32 
+    (requires fun h -> True)
+    (ensures fun h0 _ h1 -> True)
+
+let getScalar #a scalar i = 
+  push_frame(); 
+
+  let word = 
+    (* let half = logand i 0xful in  *)
+    let half = shift_right i 1ul in 
+  to_u32 (index scalar half) in 
+
+  let open Hacl.Impl.P256.Q.PrimitivesMasking in 
+  let bitShift = logand i (u64 1) in 
+    assume (uint_v bitShift == 0 \/ uint_v bitShift == 1);
+
+  let mask = to_u32 (cmovznz01  0xf0 0x0f  bitShift) in  
+  let shiftMask = to_u32 (cmovznz01  0x4 0x0 bitShift) in
+
+  let result = logand word mask in 
+  let result = shift_right result shiftMask in 
+ 
+  pop_frame();
+  result
+  
+
+
+
+[@ CInline]
+inline_for_extraction noextract  
+val montgomery_ladder_step_radix_precomputed: 
+  p: point -> tempBuffer: lbuffer uint64 (size 88) -> 
+  scalar:  lbuffer uint8 (size 32)-> 
+  i:size_t{v i < 256} -> 
+  Stack unit
+  (requires fun h -> live h p /\live h tempBuffer /\ live h scalar /\
+    LowStar.Monotonic.Buffer.all_disjoint [loc p;loc tempBuffer; loc scalar])
+  (ensures fun h0 _ h1 -> True)
+
+
+let montgomery_ladder_step_radix_precomputed p tempBuffer scalar i =  
+  let bits: uint32 = getScalar scalar (i) in 
+
+  let pointToAdd = create (size 8) (u64 0) in 
+
+  let invK h (k: nat) = True in 
+  Lib.Loops.for 0ul 16ul invK
+  (fun k -> 
+      let mask = eq_mask (to_u64 bits) (to_u64 k) in 
+      (* eq_mask_lemma d (to_u64 k);  *)
+	
+      let lut_cmb_x = Hacl.Impl.P256.Q.Comparision.global_to_comparable (sub points_radix_16 (k *! 8) (size 4)) in 
+      let lut_cmb_y = Hacl.Impl.P256.Q.Comparision.global_to_comparable (sub points_radix_16 (k *! 8 +! (size 4)) (size 4)) in 
+
+      copy_conditional (sub pointToAdd (size 0) (size 4)) lut_cmb_x mask;
+      copy_conditional (sub pointToAdd (size 4) (size 4)) lut_cmb_y mask); 
+
+
+ (*  let pointToAdd = sub points_radix_16 (bits *. size 8) (size 8) in *)
+  
+  point_double p p tempBuffer;
+  point_double p p tempBuffer;
+  point_double p p tempBuffer;
+  point_double p p tempBuffer;
+
+  
+  Hacl.Impl.P256.MixedPointAdd.point_add_mixed p pointToAdd p tempBuffer
+
+
+
+
+
+[@ CInline]
+inline_for_extraction noextract  
+val montgomery_ladder_step_radix: 
+  p: point -> tempBuffer: lbuffer uint64 (size 88) -> 
+  precomputedTable: lbuffer uint64 (size 192) ->
+  scalar:  lbuffer uint8 (size 32) -> 
+  i:size_t{v i < 256} -> 
+  Stack unit
+  (requires fun h -> live h p /\live h tempBuffer /\ live h scalar /\
+    LowStar.Monotonic.Buffer.all_disjoint [loc p;loc tempBuffer; loc scalar])
+  (ensures fun h0 _ h1 -> True)
+
+
+
+let montgomery_ladder_step_radix p tempBuffer precomputedTable scalar i =  
+  let bits = getScalar scalar i in 
+
+  let pointToAdd = create (size 12) (u64 0) in 
+
+  let invK h (k: nat) = True in 
+  Lib.Loops.for 0ul 16ul invK
+  (fun k -> 
+      let mask = eq_mask (to_u64 bits) (to_u64 k) in 
+      (* eq_mask_lemma d (to_u64 k);  *)
+	
+      let lut_cmb_x = sub precomputedTable (k *! 12) (size 4) in 
+      let lut_cmb_y = sub precomputedTable (k *! 12 +! (size 4)) (size 4) in
+      let lut_cmb_z = sub precomputedTable (k *! 12 +! (size 8)) (size 4) in 
+
+      copy_conditional (sub pointToAdd (size 0) (size 4)) lut_cmb_x mask;
+      copy_conditional (sub pointToAdd (size 4) (size 4)) lut_cmb_y mask;
+      copy_conditional (sub pointToAdd (size 8) (size 4)) lut_cmb_z mask
+      
+      
+      ); 
+      
+  
+  point_double p p tempBuffer;
+  point_double p p tempBuffer;
+  point_double p p tempBuffer;
+  point_double p p tempBuffer;
+
+  point_add pointToAdd p p tempBuffer
+
+
+
+inline_for_extraction noextract
+val montgomery_ladder_2_precomputed: #buf_type: buftype -> p: point -> 
+  scalar: lbuffer_t buf_type uint8 (size 32) -> 
+  tempBuffer:  lbuffer uint64 (size 88)  -> 
+  Stack unit
+  (requires fun h -> True )
+  (ensures fun h0 _ h1 -> modifies (loc p |+| loc tempBuffer) h0 h1)
+
+let montgomery_ladder_2_precomputed #a p scalar tempBuffer =  
+ let h0 = ST.get() in 
+
+
+
+
+  [@inline_let]
+  let spec_ml h0 = _ml_step (as_seq h0 scalar) in 
+
+  [@inline_let] 
+  let acc (h:mem) : GTot (point_nat_prime) = (fromDomainPoint(point_prime_to_coordinates (as_seq h p)))  in 
+
+  [@inline_let]
+  let inv h (i: nat {i <= 64}) = True in 
+
+ 
+  let bits: uint32 = getScalar scalar 0 in 
+  let pointToStart = sub points_radix_16 (bits *. size 8) (size 8) in 
+  let pointToStart = const_to_lbuffer pointToStart in 
+
+  copy (sub p (size 0) (size 8)) pointToStart;
+
+  upd p (size 8) (u64 1);
+  upd p (size 9) (u64 0);
+  upd p (size 10) (u64 0);
+  upd p (size 11) (u64 0);
+
+
+  for 1ul 64ul inv 
+    (fun i -> let h2 = ST.get() in
+      montgomery_ladder_step_radix_precomputed p tempBuffer scalar i
+    )
+
+inline_for_extraction noextract
+val uploadZeroPoint: p: point -> Stack unit 
+  (requires fun h -> True)
+  (ensures fun h0 _ h1 -> True)
+
+let uploadZeroPoint p = 
+  uploadZeroImpl (sub p (size 0) (size 4));
+  uploadZeroImpl (sub p (size 4) (size 4));
+  uploadZeroImpl (sub p (size 8) (size 4))
+
+
+[@ CInline]
+val generatePrecomputedTable: b: lbuffer uint64 (size 192) -> publicKey: point ->
+  tempBuffer: lbuffer uint64 (size 88) -> Stack unit  
+  (requires fun h -> True)
+  (ensures fun h0 _ h1 -> True)
+
+let generatePrecomputedTable b publicKey tempBuffer = 
+  let point0 = sub b (size 0) (size 12) in 
+  let point1 = sub b (size 12) (size 12) in 
+  let point2 = sub b (size 24) (size 12) in 
+  let point3 = sub b (size 36) (size 12) in 
+  let point4 = sub b (size 48) (size 12) in 
+  let point5 = sub b (size 60) (size 12) in 
+  let point6 = sub b (size 72) (size 12) in 
+  let point7 = sub b (size 84) (size 12) in 
+  let point8 = sub b (size 96) (size 12) in 
+  let point9 = sub b (size 108) (size 12) in 
+  let point10 = sub b (size 120) (size 12) in 
+  let point11 = sub b (size 132) (size 12) in 
+  let point12 = sub b (size 144) (size 12) in 
+  let point13 = sub b (size 156) (size 12) in 
+  let point14 = sub b (size 168) (size 12) in 
+  let point15 = sub b (size 180) (size 12) in 
+
+  uploadZeroPoint point0;
+  copy_point publicKey point1;
+  point_double publicKey point2 tempBuffer;
+  point_add point2 point1 point3 tempBuffer;
+  point_double point2 point4 tempBuffer;
+  point_add point4 point1 point5 tempBuffer;
+  point_double point3 point6 tempBuffer;
+  point_add point6 point1 point7 tempBuffer;
+  point_double point4 point8 tempBuffer;
+  point_add point8 point1 point9 tempBuffer;
+  point_double point5 point10 tempBuffer;
+  point_add point10 point1 point11 tempBuffer;
+  point_double point6 point12 tempBuffer;
+  point_add point12 point1 point13 tempBuffer;
+  point_double point7 point14 tempBuffer;
+  point_add point14 point1 point15 tempBuffer
+
+
+
+inline_for_extraction noextract
+val montgomery_ladder_2: #buf_type: buftype -> p: point -> 
+  scalar: lbuffer_t buf_type uint8 (size 32) -> 
+  tempBuffer:  lbuffer uint64 (size 88)  -> 
+  precomputedTable: lbuffer uint64 (size 192) ->
+  Stack unit
+  (requires fun h -> True )
+  (ensures fun h0 _ h1 -> modifies (loc p |+| loc tempBuffer) h0 h1)
+
+let montgomery_ladder_2 #a p scalar tempBuffer precomputedTable =  
+ let h0 = ST.get() in 
+   push_frame();
+
+     [@inline_let]
+     let spec_ml h0 = _ml_step (as_seq h0 scalar) in 
+
+     [@inline_let] 
+     let acc (h:mem) : GTot (point_nat_prime) = (fromDomainPoint(point_prime_to_coordinates (as_seq h p)))  in 
+
+     [@inline_let]
+     let inv h (i: nat {i <= 64}) = True in 
+
+     for 0ul 64ul inv 
+       (fun i -> let h2 = ST.get() in
+	 montgomery_ladder_step_radix p tempBuffer precomputedTable scalar i
+       );
+   pop_frame()
+
